# Problem 4

**Problem Statement**:  
You are given a solution \( T \) to a SubsetSum problem with set \( S = \{s_0, s_1, \ldots, s_{n-1}\} \) and a non-negative integer \( k \). The set \( T \) is a subset of \( S \) whose elements sum to \( k \), and \( s_{n-1} \in T \). Determine whether \( T' = T - \{s_{n-1}\} \) is necessarily a solution to the SubsetSum problem with inputs \( S' = \{s_0, s_1, \ldots, s_{n-2}\} \) and \( k' = k - s_{n-1} \).

---

## Solution

### 1. **Sum Calculation**  
Since \( T \) is a valid solution, we know:  
\[
\sum_{t \in T} t = k.
\]  
By removing \( s_{n-1} \) from \( T \), the sum of the new subset \( T' = T - \{s_{n-1}\} \) becomes:  
\[
\sum_{t \in T'} t = k - s_{n-1} = k'.
\]  
Thus, \( T' \) satisfies the target sum \( k' \).

---

### 2. **Subset Verification**  
- \( T \) is a subset of \( S \), and \( s_{n-1} \in T \).  
- After removing \( s_{n-1} \), \( T' \) becomes a subset of \( S' = S - \{s_{n-1}\} \).  
- Therefore, \( T' \subseteq S' \), satisfying the input constraints of the new SubsetSum problem.

---

### 3. **Edge Cases**  
- **Case 1**: If \( T = \{s_{n-1}\} \), then \( T' = \emptyset \). The sum of the empty set is \( 0 \), which matches \( k' = k - s_{n-1} = 0 \) (since \( k = s_{n-1} \)).  
- **Case 2**: If \( s_{n-1} \) is negative, \( k' = k - s_{n-1} \) could be negative. However, the SubsetSum problem allows \( k' \) to be any integer (including negatives), so \( T' \) remains valid as long as it sums to \( k' \).

---

### 4. **General Case**  
Regardless of the sign of \( s_{n-1} \):  
- \( T' \subseteq S' \) is guaranteed.  
- The sum of \( T' \) is \( k' \), which directly satisfies the requirements of the modified problem.  

---

## Conclusion  
Yes, \( T - \{s_{n-1}\} \) is always a valid solution to the SubsetSum problem with inputs \( S' \) and \( k' \).  

\[
\boxed{Yes}
\]
